ott_coq/destination_calculus_progress.v
@@ -39,7 +39,7 @@ Proof.
   - exists C, (ᵥ₎ v ⨞(λ x ⁔ m ⟼ u)). constructor.
   - exists C, (ᵥ₎ v ⨞· t'). constructor.
   - rename v into v', v0 into v, D into D2, ValidOnlyD into ValidOnlyD2. clear DestOnlyD. exists C, (ᵥ₎ v ⨞· ᵥ₎ v'). constructor.
-  - rename v into v1, Tyv into Tyv1. exists C, (ᵥ₎ hnamesᴳ(ᴳ-⁻¹ D3) ⟨ v2 ❟ v1 ⟩). constructor.
+  - rename v into v1, Tyv into Tyv1. exists C, (ᵥ₎ hnamesᴳ(D3) ⟨ v2 ❟ v1 ⟩). constructor.
   - assert (P ᴳ+ ᴳ{ x : m ‗ T} = ᴳ{ x : m ‗ T}) as elimP. { apply nDisposable_in_DestOnly; tauto. } rewrite elimP in *.
     exfalso. unfold DestOnly in DestOnlyD. specialize (DestOnlyD (ˣ x) (ₓ m ‗ T)). unfold ctx_singleton in DestOnlyD. rewrite singleton_MapsTo_at_elt in DestOnlyD. specialize (DestOnlyD eq_refl). unfold IsDest in DestOnlyD. contradiction.
   - rename Tyt into TyApp, T into U, T0 into T, t0 into t, Tyt0 into Tyt, P1 into D1, P2 into D2.
@@ -68,7 +68,7 @@ Proof.
   - rename Tyt into TyMap, t0 into t, Tyt0 into Tyt, P1 into D1, P2 into D2. destruct (NotVal_dec t).
     * destruct e; subst. rename x0 into v. inversion Tyt; subst. inversion Tyv; subst. { exfalso. apply Ty_val_Hole_DestOnly_contra with (D := ᴳ{+ h : U ⧔ T ‗ ¹ν}) (h := h) (T := U ⧔ T); tauto. }
       rename D2 into D', D0 into D2. assert (DestOnly (P ᴳ+ (D1 ᴳ+ D2))) as DestOnlyPuD1uD2. { crush. } rewrite (nDisposable_in_DestOnly P (D1 ᴳ+ D2) DisposP DestOnlyPuD1uD2) in *.
-      exists (C ∘ hnamesᴳ(ᴳ-⁻¹ D3) ᴴ⩲ (maxᴴ(hnames©(C)) + 1) ᵒᵖ⟨ v2 ᵛ[hnamesᴳ(ᴳ-⁻¹ D3) ⩲ (maxᴴ(hnames©(C)) + 1)] ❟⬜⟩), (t' ᵗ[x ≔ v1 ᵛ[hnamesᴳ(ᴳ-⁻¹ D3) ⩲ (maxᴴ(hnames©(C)) + 1)]]). constructor; tauto.
+      exists (C ∘ hnamesᴳ(D3) ᴴ⩲ (maxᴴ(hnames©(C)) + 1) ᵒᵖ⟨ v2 ᵛ[hnamesᴳ( D3) ⩲ (maxᴴ(hnames©(C)) + 1)] ❟⬜⟩), (t' ᵗ[x ≔ v1 ᵛ[hnamesᴳ( D3) ⩲ (maxᴴ(hnames©(C)) + 1)]]). constructor; tauto.
     * exists (C ∘ ⬜map x ⟼ t'), t. constructor; tauto.
   - rename Tyt into TyToA. destruct (NotVal_dec u).
     * destruct e; subst. rename x into v2. exists C, (ᵥ₎ HNames.empty ⟨ v2 ❟ ᵛ() ⟩ ). constructor.
@@ -96,7 +96,7 @@ Proof.
         - assumption.
         - crush. }
       apply union_empty_iff in Empty. destruct Empty as [_ EmptyD3].
-      subst. rewrite hnames_minus_eq, hnames_empty_is_hempty.
+      subst. rewrite hnames_empty_is_hempty.
       exists C, (ᵥ₎ ᵛ( v2 , ᴇ ¹∞ ⁔ v' )). constructor.
     * exists (C ∘ from⧔⬜), t. constructor; tauto.
   - rename Tyt into TyFillU, Tyt0 into Tyt, t0 into t. destruct (NotVal_dec t).
@@ -127,8 +127,8 @@ Proof.
     * destruct e; subst. rename x into v. destruct (NotVal_dec t').
       + destruct e; subst. rename x into v'. inversion Tyt; subst. inversion Tyv; subst. { exfalso. apply Ty_val_Hole_DestOnly_contra with (D := ᴳ{+ h : ⌊ U ⌋ n ‗ ¹ν}) (h := h) (T := ⌊ U ⌋ n); tauto. } rename H1 into DestOnlyD'. inversion Tytp; subst. rename Tyv0 into Tyvp. inversion Tyvp; subst. { exfalso. apply Ty_val_Hole_DestOnly_contra with (D := ᴳ{+ h0 : U ⧔ T ‗ ¹ν}) (h := h0) (T := U ⧔ T); tauto. } assert (DestOnly (P0 ᴳ+ (D1 ᴳ+ D2))) as DestOnlyP0uD1uD2. { crush. } rewrite (nDisposable_in_DestOnly P0 (D1 ᴳ+ D2) DisposP0 DestOnlyP0uD1uD2) in *.
       exists
-        ( C ©️[ h ≔ hnamesᴳ(ᴳ-⁻¹ D3) ᴴ⩲ (maxᴴ( hnames©(C) ∪ ᴴ{ h}) + 1) ‗  v2 ᵛ[hnamesᴳ(ᴳ-⁻¹ D3) ⩲ (maxᴴ( hnames©(C) ∪ ᴴ{ h}) + 1)] ] ),
-        (ᵥ₎ v1 ᵛ[hnamesᴳ(ᴳ-⁻¹ D3) ⩲ (maxᴴ( hnames©(C) ∪ ᴴ{ h}) + 1)]).
+        ( C ©️[ h ≔ hnamesᴳ( D3) ᴴ⩲ (maxᴴ( hnames©(C) ∪ ᴴ{ h}) + 1) ‗  v2 ᵛ[hnamesᴳ( D3) ⩲ (maxᴴ( hnames©(C) ∪ ᴴ{ h}) + 1)] ] ),
+        (ᵥ₎ v1 ᵛ[hnamesᴳ( D3) ⩲ (maxᴴ( hnames©(C) ∪ ᴴ{ h}) + 1)]).
       constructor; tauto.
       + exists (C ∘ v ⨞·⬜), t'. constructor; tauto.
     * exists (C ∘ ⬜⨞· t'), t. constructor; tauto.
